Add stores with updatable environments.

src/Env.v
@@ -2,8 +2,8 @@
 (** * Typing Environments *)
 
 From Coq Require Import Program Program.Tactics ZArith.
-From mathcomp Require Import ssreflect ssrbool eqtype.
-From ssrlib Require Import HList Var ZAriths.
+From mathcomp Require Import ssreflect ssrbool eqtype seq.
+From ssrlib Require Import Types SsrOrdered FSets FMaps HList Var ZAriths.
 
 Set Implicit Arguments.
 Unset Strict Implicit.
@@ -11,64 +11,272 @@ Import Prenex Implicits.
 
 
 
-(** Environments for variables with the same type. *)
+(** Environments for variables with the same type *)
 
-Module SEnv.
+Module Type SEnv.
+
+  Declare Module V : SsrOrderedType.
+
+  (* The type of environments *)
+  Parameter t : Type.
+
+  (* An empty environment *)
+  Parameter empty : t.
+
+  (* Check if a variable is defined in an environment *)
+  Parameter mem : V.t -> t -> bool.
+  Axiom mem_empty : forall (x : V.t), mem x empty = false.
+
+  (* Add a variable to an environment *)
+  Parameter add : V.t -> t -> t.
+  Axiom mem_add_eq :
+    forall (E : t) (x : V.t), mem x (add x E).
+  Axiom mem_add_neq :
+    forall (E : t) (x y : V.t), x != y -> mem x (add y E) = mem x E.
+
+  (* Variables in an environment *)
+  Parameter pvar : t -> Type.
+  Parameter make_pvar : forall (E : t) (x : V.t), mem x E -> pvar E.
+  Parameter pvar_var : forall (E : t), pvar E -> V.t.
+  Axiom pvar_var_mem :
+    forall (E : t) (x : pvar E), mem (pvar_var x) E.
+
+  (* Creating new variables *)
+  Parameter new_var : t -> V.t.
+  Axiom new_var_is_new : forall (E : t), ~~ mem (new_var E) E.
+
+End SEnv.
+
+
+
+Module MakeSEnv (V : SsrOrderedWithDefaultSucc) <: SEnv with Module V := V.
+
+  Module V := V.
+
+  Local Notation var := V.t.
+
+  Module VS := MakeTreeSetWithNew V.
 
   Definition t : Type := VS.t.
 
   Definition empty : t := VS.empty.
 
-  (* Check if a variable is defined in an environment. *)
   Definition mem (v : var) (E : t) : bool := VS.mem v E.
+
+  Lemma mem_empty : forall (x : V.t), mem x empty = false.
+  Proof.
+    move=> x. exact: VS.Lemmas.mem_empty.
+  Qed.
 
   Definition add (v : var) (E : t) : t := VS.add v E.
 
-  Inductive pvar (E : t) : Set :=
-  | PVar : forall x : var, VS.mem x E -> pvar E.
+  Lemma mem_add_eq :
+    forall (E : t) (x : V.t), mem x (add x E).
+  Proof.
+    move=> E x. apply: VS.Lemmas.mem_add_eq. exact: eqxx.
+  Qed.
+
+  Lemma mem_add_neq :
+    forall (E : t) (x y : V.t), x != y -> mem x (add y E) = mem x E.
+  Proof.
+    move=> E x y Hne. apply: VS.Lemmas.mem_add_neq. apply/negP. exact: Hne.
+  Qed.
+
+  Inductive pvar_t (E : t) : Type :=
+  | PVar : forall x : V.t, VS.mem x E -> pvar_t E.
+
+  Definition pvar := pvar_t.
+
+  Definition make_pvar := PVar.
 
   Definition pvar_var (E : t) (x : pvar E) : var :=
     match x with
     | PVar v _ => v
     end.
 
-  (* Create a new variable. *)
+  Lemma pvar_var_mem :
+    forall (E : t) (x : pvar E), mem (pvar_var x) E.
+  Proof.
+    move=> E []. done.
+  Qed.
 
-  Definition new_var (E : t) : var := VS.new_var E.
+  Definition new_var (E : t) : var := VS.new_elt E.
 
   Lemma new_var_is_new :
     forall (E : t), ~~ mem (new_var E) E.
   Proof.
-    exact: VS.new_var_is_new.
+    exact: VS.new_elt_is_new.
   Qed.
 
-End SEnv.
+End MakeSEnv.
 
 
 
-(** Environments for variables with heterogeneous types. *)
+(** Environments for variables with heterogeneous types *)
 
-Module TEnv.
+Module Type TEnv.
+
+  Declare Module V : SsrOrderedType.
+
+  Section Env.
+
+    (* Types *)
+    Variable T : Type.
+
+    (* Environments *)
+    Parameter t : Type -> Type.
+
+    (* An empty environment *)
+    Parameter empty : t T.
+
+    (* Check if a variable is defined in an environment *)
+    Parameter mem : V.t -> t T -> bool.
+    Axiom mem_empty : forall (x : V.t), mem x empty = false.
+
+    (* Find the type of a variable in an environment *)
+    Parameter find : V.t -> t T -> option T.
+    Axiom find_some_mem :
+      forall (E : t T) (x : V.t) (ty : T),
+        find x E = Some ty -> mem x E.
+    Axiom find_none_not_mem :
+      forall (E : t T) (x : V.t),
+        find x E = None -> mem x E = false.
+    Axiom mem_find_some :
+      forall (E : t T) (x : V.t),
+        mem x E -> exists (ty : T), find x E = Some ty.
+    Axiom not_mem_find_none :
+      forall (E : t T) (x : V.t),
+        mem x E = false -> find x E = None.
+
+    (* Add a variable to an environment *)
+    Parameter add : V.t -> T -> t T -> t T.
+    Axiom mem_add_eq :
+      forall (E : t T) (x : V.t) (ty : T), mem x (add x ty E).
+    Axiom mem_add_neq :
+      forall (E : t T) (x y : V.t) (ty : T), x != y -> mem x (add y ty E) = mem x E.
+    Axiom find_add_eq :
+      forall (E : t T) (x : V.t) (ty : T),
+        find x (add x ty E) = Some ty.
+    Axiom find_add_neq :
+      forall (E : t T) (x y : V.t) (ty : T),
+        x != y -> find x (add y ty E) = find x E.
+
+    (* Variables in an environment *)
+    Parameter pvar : t T -> Type.
+    Parameter make_pvar :
+      forall (E : t T) (x : V.t) (ty : T),
+        find x E = Some ty -> pvar E.
+    Parameter pvar_var : forall (E : t T), pvar E -> V.t.
+    Parameter pvar_ty : forall (E : t T), pvar E -> T.
+    Axiom pvar_var_mem :
+      forall (E : t T) (x : pvar E), mem (pvar_var x) E.
+    Axiom pvar_ty_find :
+      forall (E : t T) (x : pvar E), find (pvar_var x) E = Some (pvar_ty x).
+
+    (* Creating new variables *)
+    Parameter new_var : t T -> V.t.
+    Axiom new_var_is_new : forall (E : t T), ~~ mem (new_var E) E.
+
+  End Env.
+
+End TEnv.
+
+
+
+Module MakeTEnv (Import V : SsrOrderedWithDefaultSucc) <: TEnv with Module V := V.
+
+  Module V := V.
+
+  Local Notation var := V.t.
+
+  Module VM := MakeTreeMapWithNew V.
 
   Section Env.
 
     (* Variable types. *)
-    Variable T : Set.
+    Variable T : Type.
 
     Definition t : Type := VM.t T.
 
     Definition empty : t := VM.empty T.
 
-    (* Check if a variable is defined in an environment. *)
+    (* Check if a variable is defined in an environment *)
     Definition mem (v : var) (E : t) : bool := VM.mem v E.
 
-    (* Find the type of a variable in an environment. *)
+    Lemma mem_empty : forall (x : var), mem x empty = false.
+    Proof.
+      exact: VM.Lemmas.empty_a.
+    Qed.
+
+    (* Find the type of a variable in an environment *)
     Definition find (v : var) (E : t) : option T := VM.find v E.
 
+    Lemma find_some_mem :
+      forall (E : t) (x : var) (ty : T),
+        find x E = Some ty -> mem x E.
+    Proof.
+      exact: VM.Lemmas.find_some_mem.
+    Qed.
+
+    Lemma find_none_not_mem :
+      forall (E : t) (x : var),
+        find x E = None -> mem x E = false.
+    Proof.
+      exact: VM.Lemmas.find_none_not_mem.
+    Qed.
+
+    Lemma mem_find_some :
+      forall (E : t) (x : var),
+        mem x E -> exists (ty : T), find x E = Some ty.
+    Proof.
+      exact: VM.Lemmas.mem_find_some.
+    Qed.
+
+    Lemma not_mem_find_none :
+      forall (E : t) (x : var),
+        mem x E = false -> find x E = None.
+    Proof.
+      move=> E x. move/idP/negP. exact: VM.Lemmas.not_mem_find_none.
+    Qed.
+
+    (* Add a variable to an environment *)
     Definition add (v : var) (ty : T) (E : t) : t := VM.add v ty E.
 
-    Inductive pvar (E : t) : Set :=
-    | PVar : forall (x : var) (ty : T), find x E = Some ty -> pvar E.
+    Lemma mem_add_eq :
+      forall (E : t) (x : var) (ty : T), mem x (add x ty E).
+    Proof.
+      move=> E x t. exact: VM.Lemmas.add_eq_b.
+    Qed.
+
+    Lemma mem_add_neq :
+      forall (E : t) (x y : var) (ty : T), x != y -> mem x (add y ty E) = mem x E.
+    Proof.
+      move=> E x y t Hne. apply: VM.Lemmas.add_neq_b. move=> H. move/eq_sym: H.
+      apply/negP. assumption.
+    Qed.
+
+    Lemma find_add_eq :
+      forall (E : t) (x : var) (ty : T),
+        find x (add x ty E) = Some ty.
+    Proof.
+      move=> E x y. exact: VM.Lemmas.add_eq_o.
+    Qed.
+
+    Lemma find_add_neq :
+      forall (E : t) (x y : var) (ty : T),
+        x != y -> find x (add y ty E) = find x E.
+    Proof.
+      move=> E x y t Hne. apply: VM.Lemmas.add_neq_o. move=> H. move/eq_sym: H.
+      apply/negP. assumption.
+    Qed.
+
+    (* Variables in an environment *)
+    Inductive pvar_t (E : t) : Type :=
+    | PVar : forall (x : var) (ty : T), find x E = Some ty -> pvar_t E.
+
+    Definition pvar := pvar_t.
+
+    Definition make_pvar := PVar.
 
     Definition pvar_var (E : t) (x : pvar E) : var :=
       match x with
@@ -80,253 +288,563 @@ Module TEnv.
       | PVar _ ty _ => ty
       end.
 
-    (* Create a new variable. *)
+    Lemma pvar_var_mem :
+      forall (E : t) (x : pvar E), mem (pvar_var x) E.
+    Proof.
+      move=> E [] x t H /=. exact: (find_some_mem H).
+    Qed.
 
-    Definition new_var (E : t) : var := VM.new_var E.
+    Lemma pvar_ty_find :
+      forall (E : t) (x : pvar E), find (pvar_var x) E = Some (pvar_ty x).
+    Proof.
+      move=> E [] x t H /=. assumption.
+    Qed.
+
+    (* Creating new variables *)
+    Definition new_var (E : t) : VM.key := VM.new_key E.
 
     Lemma new_var_is_new :
       forall (E : t), ~~ mem (new_var E) E.
     Proof.
-      exact: VM.new_var_is_new.
-    Qed.
-
-    (* Convert to SEnv. *)
-
-    Definition to_senv (E : t) : SEnv.t := VM.vset E.
-
-    Lemma mem_to_senv E :
-      forall x, mem x E -> SEnv.mem x (to_senv E).
-    Proof.
-      exact: VM.mem_vset.
+      exact: VM.new_key_is_new.
     Qed.
 
   End Env.
 
-End TEnv.
+End MakeTEnv.
 
 
 
 (** Environments for variables with heterogeneous types. Indices for the access
  of values in a heterogeneous list (HList) are defined in the environments. *)
 
-Module HEnv.
+Module Type HEnv.
+
+  Declare Module V : SsrOrderedType.
 
   Section Env.
 
-  Local Open Scope hlist_scope.
+    Local Open Scope hlist_scope.
 
-  (* Variable type. *)
-  Variable T : Set.
+    (* Types *)
+    Variable T : Type.
 
-  Record entry (types : list T) := mkEntry { vty : T;
-                                             vin: bool;
-                                             vidx : lidx vty types }.
+    (* Entry *)
+    Parameter entry : list T -> Type.
+    Parameter vty : forall types : list T, entry types -> T.
+    Parameter vidx : forall (types : list T) (e : entry types), lidx (vty e) types.
 
-  Record t := mkEnv { vtypes : list T;
-                      vmap : VM.t (entry vtypes);
-                      lidx_disjoint :
-                        forall (x y : var) (ex ey : entry vtypes),
-                          VM.find x vmap = Some ex ->
-                          VM.find y vmap = Some ey ->
-                          x != y ->
-                          vidx ex <>i vidx ey }.
+    (* Environments *)
+    Parameter t : Type -> Type.
+    Parameter vtypes : t T -> list T.
 
-  Program Definition empty : t := {| vtypes := nil;
-                                     vmap := VM.empty (entry nil) |}.
+    (* An empty environment *)
+    Parameter empty : t T.
+    Axiom vtypes_empty : vtypes empty = [::].
 
-  (* Check if a variable is defined in an environment. *)
-  Definition mem (v : var) (E : t) : bool := VM.mem v (vmap E).
+    (* Check if a variable is defined in an environment *)
+    Parameter mem : V.t -> t T -> bool.
+    Axiom mem_empty : forall x, mem x empty = false.
 
-  (* Find the entry of a variable in an environment. *)
-  Definition find (v : var) (E : t) : option (entry (vtypes E)) :=
-    VM.find v (vmap E).
+    (* Find the type of a variable in an environment *)
+    Parameter find : V.t -> forall (E : t T), option (entry (vtypes E)).
+    Parameter find_ty : V.t -> t T -> option T.
+    Parameter find_idx :
+      (forall (x y : T), {x = y} + {x <> y}) ->
+      forall (v : V.t) (ty : T) (E : t T), option (lidx ty (vtypes E)).
 
-  (* Find the type of a variable in an environment. *)
-  Definition find_type (v : var) (E : t) : option T :=
-    match find v E with
-    | None => None
-    | Some e => Some (vty e)
-    end.
+    Axiom find_none_find_ty_none :
+      forall (E : t T) (x : V.t), find x E = None -> find_ty x E = None.
+    Axiom find_some_find_ty_some :
+      forall (E : t T) (x : V.t) e,
+        find x E = Some e -> find_ty x E = Some (vty e).
 
-  (* Prepend a vtype to an entry. *)
-  Definition prepend_vtype_to_entry {ty : T} {types : list T} (e : entry types) : entry (ty::types) :=
-    {| vty := vty e;
-       vin := vin e;
-       vidx := HIS ty (vidx e) |}.
+    (* Failed to prove *)
+    (*
+    Axiom find_some_find_idx_some :
+      forall (E : t T) (x : V.t) (ty : T) e,
+        find x E = Some e /\ vty e = ty -> find_idx x ty E ~= Some (vty e).
+    *)
+    Axiom find_none_find_idx_none :
+      forall (ty_dec : forall (x y : T), {x = y} + {x <> y}),
+      forall (E : t T) (x : V.t) (ty : T), find x E = None -> find_idx ty_dec x ty E = None.
 
-  (* Prepend a vtype to the list of variable types of an environment. *)
-  Definition prepend_vtype (ty : T) (types : list T)
-             (m : VM.t (entry types)) : VM.t (entry (ty::types)) :=
-    VM.map (prepend_vtype_to_entry (ty:=ty) (types:=types)) m.
+    Axiom find_some_mem :
+      forall (E : t T) (x : V.t) e,
+        find x E = Some e -> mem x E.
+    Axiom find_none_not_mem :
+      forall (E : t T) (x : V.t),
+        find x E = None -> mem x E = false.
 
-  (* Declare a program variable in an environment. *)
-  Program Definition add_var (v : var) (ty : T) (input : bool) (E : t) : t :=
-    {| vtypes := ty::(vtypes E);
-       vmap := VM.add v {| vty := ty; vin := input; vidx := HI0 ty (vtypes E) |}
-                      (prepend_vtype ty (vmap E)) |}.
-  Next Obligation.
-    case Hxv: (x == v); move/idP: Hxv => Hxv.
-    - (* x == v *)
-      case Hyv: (y == v); move/idP: Hyv => Hyv.
-      + (* y == v *)
-        rewrite (eqP Hxv) (eqP Hyv) in H1.
-        apply: False_ind; apply: (negP H1); reflexivity.
-      + (* y != v *)
-        rewrite (VM.Lemmas.find_add_eq _ _ (Hxv)) in H;
-        rewrite (VM.Lemmas.find_add_neq _ _ Hyv) /prepend_vtype in H0 =>
-        {H1 Hxv Hyv}.
-        case: H => H; rewrite -H /= => {H}.
-        move: (VM.Lemmas.find_map_some H0) => {H0} [ey' [He_ey _]].
-        rewrite He_ey /prepend_vtype_to_entry /=.
-        move=> Heq; by inversion Heq.
-    - (* x != v *)
-      rewrite (VM.Lemmas.find_add_neq _ _ Hxv) /prepend_vtype in H => {Hxv}.
-      move: (VM.Lemmas.find_map_some H) => {H} [ex' [He_ex He_x]].
-      rewrite He_ex /prepend_vtype_to_entry /= => {He_ex}.
-      case Hyv: (y == v); move/idP: Hyv => Hyv.
-      + (* y == v *)
-        rewrite (VM.Lemmas.find_add_eq _ _ Hyv) in H0 => {Hyv}.
-        case: H0 => H0; rewrite -H0 /= => {H0}.
-        move=> Heq; by inversion Heq.
-      + (* y != v *)
-        rewrite (VM.Lemmas.find_add_neq _ _ Hyv) /prepend_vtype in H0 => {Hyv}.
-        move: (VM.Lemmas.find_map_some H0) => {H0} [ey' [He_ey He_y]].
-        rewrite He_ey /prepend_vtype_to_entry /= => {He_ey}.
-        move: (lidx_disjoint He_x He_y H1) => Hne Heq; apply: Hne.
-        exact: (his_eq_lidx_eq Heq).
-  Qed.
+    Axiom mem_find_some :
+      forall (E : t T) (x : V.t),
+        mem x E -> exists e, find x E = Some e.
+    Axiom not_mem_find_none :
+      forall (E : t T) (x : V.t),
+        mem x E = false -> find x E = None.
 
-  (* Declare an input variable in an environment. *)
-  Definition add_input (v : var) (ty : T) (E : t) : t :=
-    add_var v ty true E.
+    (* Prepend a vtype to an entry *)
+    Parameter prepend_vtype :
+      forall (ty : T) (types : list T), entry types -> entry (ty::types).
+    Axiom prepend_vtype_vty :
+      forall (ty : T) (types : list T) (e : entry types),
+        vty (prepend_vtype ty e) = vty e.
+    Axiom prepend_vtype_vidx :
+      forall (ty : T) (types : list T) (e : entry types),
+        vidx (prepend_vtype ty e) ~= HIS ty (vidx e).
 
-  (* Declare a local variable in an environment. *)
-  Definition add_local (v : var) (ty : T) (E : t) : t :=
-    add_var v ty false E.
+    (* Add a variable to an environment *)
+    Parameter add : V.t -> T -> t T -> t T.
+    Axiom mem_add_eq :
+      forall (E : t T) (x : V.t) (ty : T), mem x (add x ty E).
+    Axiom mem_add_neq :
+      forall (E : t T) (x y : V.t) (ty : T), x != y -> mem x (add y ty E) = mem x E.
+    Axiom find_add_heq :
+      forall (E : t T) (x : V.t) (ty : T),
+        (exists e : entry (ty::(vtypes E)),
+            find x (add x ty E) ~= Some e /\
+            vty e = ty /\
+            lidx_eq (vidx e) (HI0 ty (vtypes E))).
+    Axiom find_add_eq :
+      forall (E : t T) (x : V.t) (ty : T),
+        (exists e : entry (vtypes (add x ty E)),
+            find x (add x ty E) = Some e /\
+            vty e = ty /\
+            (vidx e) ~= (HI0 ty (vtypes E))).
+    Axiom find_ty_add_eq :
+      forall (E : t T) (x : V.t) (ty : T),
+        find_ty x (add x ty E) = Some ty.
+    Axiom find_ty_add_neq :
+      forall (E : t T) (x y : V.t) (ty : T),
+        x != y -> find_ty x (add y ty E) = find_ty x E.
+    Axiom find_add_neq :
+      forall (E : t T) (x y : V.t) (ty : T),
+        x != y ->
+        find x (add y ty E) ~= match find x E with
+                              | None => None
+                              | Some e => Some (prepend_vtype ty e)
+                              end.
+    Axiom vtypes_add :
+      forall (E : t T) (x : V.t) (ty : T),
+        vtypes (add x ty E) = ty::(vtypes E).
 
-  (* A pvar is a variable of a specified type defined in an environment. *)
-  (* Note: The equality of vtypes used here is =, not ==. If == is used, then
-   * we will fail to do dependent destruction.
-   *)
-  Inductive pvar (E : t) (ty : T) : Set :=
-  | PVar : forall v e, find v E = Some e -> vty e = ty -> pvar E ty.
+    (* Variables in an environment *)
+    Parameter pvar : t T -> T -> Type.
+    Parameter make_pvar :
+      forall (E : t T) (ty : T) (v : V.t) (e : entry (vtypes E)),
+        find v E = Some e -> vty e = ty -> pvar E ty.
+    Parameter pvar_var : forall (E : t T) (ty : T), pvar E ty -> V.t.
+    Parameter pvar_lidx : forall (E : t T) (ty : T), pvar E ty -> lidx ty (vtypes E).
+    Axiom pvar_var_mem :
+      forall (E : t T) (ty : T) (x : pvar E ty), mem (pvar_var x) E.
+    Axiom pvar_vtype_eq :
+      forall (E : t T) (ty1 ty2 : T) (x : pvar E ty1) (y : pvar E ty2),
+        pvar_var x == pvar_var y -> ty1 = ty2.
+    Axiom pvar_lidx_heq :
+      forall (E : t T) (ty1 ty2 : T) (x : pvar E ty1) (y : pvar E ty2),
+        pvar_var x == pvar_var y -> (pvar_lidx x =i pvar_lidx y)%hlist.
+    Axiom pvar_lidx_eq :
+      forall (E : t T) (ty : T) (x y : pvar E ty),
+        pvar_var x == pvar_var y -> pvar_lidx x = pvar_lidx y.
+    Axiom pvar_lidx_hneq :
+      forall (E : t T) (ty1 ty2 : T) (x : pvar E ty1) (y : pvar E ty2),
+        pvar_var x != pvar_var y -> pvar_lidx x <>i pvar_lidx y.
 
-  (* A any_pvar is a defined variable in an environment. *)
-  Inductive any_pvar (E : t) : Set :=
-  | AnyPVar : forall (v : var) (ty : T), pvar E ty -> any_pvar E.
-
-  (* Return the variable ID of a pvar. *)
-  Definition pvar_var (E : t) ty (x : pvar E ty) : var :=
-    match x with
-    | PVar v _ _ _ => v
-    end.
-
-  (* Return the entry of a pvar in an environment. *)
-  Definition pvar_entry (E : t) ty (x : pvar E ty) : entry (vtypes E) :=
-    match x with
-    | PVar _ e _ _ => e
-    end.
-
-  (* Return the lidx of a pvar in an environment. *)
-  Program Definition pvar_lidx (E : t) ty (x : pvar E ty) : lidx ty (vtypes E) :=
-    match x with
-    | PVar _ e _ _ => Env.vidx e
-    end.
-
-  (* Lemmas about pvar. *)
-
-  Lemma pvar_vtype_eq (E : t) (ty1 ty2 : T) (x : pvar E ty1) (y : pvar E ty2) :
-    pvar_var x == pvar_var y -> ty1 = ty2.
-  Proof.
-    elim: x => x ex Hex Htx /=.
-    elim: y => y ey Hey Hty /=.
-    move/eqP=> Hxy.
-    rewrite -Hxy Hex in Hey.
-    case: Hey => Hexey; rewrite -Hexey Htx in Hty.
-    exact: Hty.
-  Qed.
-
-  Lemma pvar_lidx_heq (E : t) (tyx tyy : T) (x : pvar E tyx) (y : pvar E tyy) :
-    pvar_var x == pvar_var y -> (pvar_lidx x =i pvar_lidx y)%hlist.
-  Proof.
-    elim: x => x ex Hex Htx /=.
-    elim: y => y ey Hey Hty /=.
-    move/eqP=> Hxy.
-    dependent destruction Htx.
-    dependent destruction Hty.
-    rewrite /=.
-    rewrite -Hxy Hex in Hey.
-    case: Hey => Hey; rewrite Hey.
-    reflexivity.
-  Qed.
-
-  Lemma pvar_lidx_eq (E : t) ty (x y : pvar E ty) :
-    pvar_var x == pvar_var y -> pvar_lidx x = pvar_lidx y.
-  Proof.
-    move=> Hxy.
-    apply: lidx_eq_eq.
-    apply: pvar_lidx_heq.
-    assumption.
-  Qed.
-
-  Lemma pvar_lidx_hneq (E : t) (tyx tyy : T) (x : pvar E tyx) (y : pvar E tyy) :
-    pvar_var x != pvar_var y -> pvar_lidx x <>i pvar_lidx y.
-  Proof.
-    elim: x => x ex Hex Htx.
-    elim: y => y ey Hey Hty.
-    move=> /= Hne.
-    dependent destruction Htx.
-    dependent destruction Hty.
-    rewrite /=.
-    apply: (lidx_disjoint Hex Hey).
-    assumption.
-  Qed.
-
-  (* Create a new variable. *)
-
-  Definition new_var (E : t) : var := VM.new_var (vmap E).
-
-  Lemma new_var_is_new :
-    forall (E : t), ~~ mem (new_var E) E.
-  Proof.
-    move=> E.
-    exact: (VM.new_var_is_new (vmap E)).
-  Qed.
-
-  (* Convert to SEnv. *)
-
-  Definition to_senv (E : t) : SEnv.t := VM.vset (vmap E).
-
-  Lemma mem_to_senv E :
-    forall x, mem x E -> SEnv.mem x (to_senv E).
-  Proof.
-    exact: VM.mem_vset.
-  Qed.
-
-  (* Convert to TEnv. *)
-
-  Definition to_tenv (E : t) : TEnv.t T :=
-    VM.map (vty (types:=vtypes E)) (vmap E).
-
-  Lemma mem_to_tenv E :
-    forall x, mem x E -> TEnv.mem x (to_tenv E).
-  Proof.
-    rewrite /TEnv.mem /to_tenv => x Hmem.
-    rewrite VM.Lemmas.map_b.
-    exact: Hmem.
-  Qed.
-
-  Lemma to_tenv_find_ty (E : t) :
-    forall x, find_type x E = TEnv.find x (to_tenv E).
-  Proof.
-    rewrite /find_type /find /TEnv.find /to_tenv => x.
-    case H: (VM.find x (vmap E)).
-    - apply: Logic.eq_sym.
-      exact: (VM.Lemmas.find_some_map _ H).
-    - apply: Logic.eq_sym.
-      exact: (VM.Lemmas.find_none_map _ H).
-  Qed.
+    (* Creating new variables *)
+    Parameter new_var : t T -> V.t.
+    Axiom new_var_is_new : forall (E : t T), ~~ mem (new_var E) E.
 
   End Env.
 
 End HEnv.
+
+
+Module MakeHEnv (V : SsrOrderedWithDefaultSucc) <: HEnv with Module V := V.
+
+  Module V := V.
+  Module VM := MakeTreeMapWithNew V.
+
+  Local Notation var := V.t.
+
+  Section Env.
+
+    Local Open Scope hlist_scope.
+
+    (* Types *)
+    Variable T : Type.
+
+    Variable ty_dec : forall (x y : T), {x = y} + {x <> y}.
+
+    Record entry_t (types : list T) := mkEntry { vty : T;
+                                                 vidx : lidx vty types }.
+
+    Definition entry := entry_t.
+
+    (* Environments *)
+    Record t_t := mkEnv { vtypes : list T;
+                          vmap : VM.t (entry vtypes);
+                          lidx_disjoint :
+                            forall (x y : var) (ex ey : entry vtypes),
+                              VM.find x vmap = Some ex ->
+                              VM.find y vmap = Some ey ->
+                              x != y ->
+                              vidx ex <>i vidx ey }.
+
+    Definition t := t_t.
+    Definition make_env := mkEnv.
+
+    (* An empty environment *)
+    Program Definition empty : t := {| vtypes := nil;
+                                       vmap := VM.empty (entry nil) |}.
+    Lemma vtypes_empty : vtypes empty = [::].
+    Proof.
+      reflexivity.
+    Qed.
+
+    (* Check if a variable is defined in an environment *)
+    Definition mem (v : var) (E : t) : bool := VM.mem v (vmap E).
+
+    Lemma mem_empty : forall x, mem x empty = false.
+    Proof.
+      exact: VM.Lemmas.empty_a.
+    Qed.
+
+    (* Find the entry of a variable in an environment *)
+    Definition find (v : var) (E : t) : option (entry (vtypes E)) :=
+      VM.find v (vmap E).
+
+    (* Find_idx cannot be defined in the following way. *)
+    (*
+    Program Definition find_idx (v : var) (E : t) :=
+      match find v E with
+      | None => None
+      | Some e => Some e
+      end.
+    *)
+
+    Program Definition find_idx (v : var) (ty : T) (E : t) : option (lidx ty (vtypes E)) :=
+      match find v E with
+      | None => None
+      | Some e => match ty_dec ty (vty e) with
+                  | left _ => Some (vidx e)
+                  | right _ => None
+                  end
+      end.
+
+    (* Find the type of a variable in an environment. *)
+    Definition find_ty (v : var) (E : t) : option T :=
+      match find v E with
+      | None => None
+      | Some e => Some (vty e)
+      end.
+
+    Lemma find_none_find_ty_none :
+      forall (E : t) (x : var), find x E = None -> find_ty x E = None.
+    Proof.
+      rewrite /find_ty => E x ->. reflexivity.
+    Qed.
+
+    Lemma find_some_find_ty_some :
+      forall (E : t) (x : var) e,
+        find x E = Some e -> find_ty x E = Some (vty e).
+    Proof.
+      rewrite /find_ty => E x e ->. reflexivity.
+    Qed.
+
+    Lemma find_none_find_idx_none :
+      forall (E : t) (x : var) (ty : T), find x E = None -> find_idx x ty E = None.
+    Proof.
+      move=> E x ty H. rewrite /find_idx. rewrite H. reflexivity.
+    Qed.
+
+    Lemma find_some_find_idx_some :
+      forall (E : t) (x : var) (ty : T) (e : entry (vtypes E)),
+        find x E = Some e /\ vty e = ty -> find_idx x ty E ~= Some (vty e).
+    Proof.
+      move=> E x ty e [Hfind Hty]. rewrite /find_idx Hfind /=.
+      (* Does not know how to proceed *)
+    Abort.
+
+    Lemma find_some_mem :
+      forall (E : t) (x : var) e,
+        find x E = Some e -> mem x E.
+    Proof.
+      move=> E x e H. exact: (VM.Lemmas.find_some_mem H).
+    Qed.
+
+    Lemma find_none_not_mem :
+      forall (E : t) (x : var),
+        find x E = None -> mem x E = false.
+    Proof.
+      move=> E x H. exact: (VM.Lemmas.find_none_not_mem H).
+    Qed.
+
+    Lemma mem_find_some :
+      forall (E : t) (x : var),
+        mem x E -> exists e, find x E = Some e.
+    Proof.
+      move=> E x H. exact: (VM.Lemmas.mem_find_some).
+    Qed.
+
+    Lemma not_mem_find_none :
+      forall (E : t) (x : var),
+        mem x E = false -> find x E = None.
+    Proof.
+      move=> E x. move/idP/negP. exact: (VM.Lemmas.not_mem_find_none).
+    Qed.
+
+    (* Prepend a vtype to an entry *)
+    Definition prepend_vtype (ty : T) {types : list T} (e : entry types) : entry (ty::types) :=
+      {| vty := vty e;
+         vidx := HIS ty (vidx e) |}.
+
+    Lemma prepend_vtype_vty :
+      forall (ty : T) (types : list T) (e : entry types),
+        vty (prepend_vtype ty e) = vty e.
+    Proof.
+      reflexivity.
+    Qed.
+
+    Lemma prepend_vtype_vidx :
+      forall (ty : T) (types : list T) (e : entry types),
+        vidx (prepend_vtype ty e) ~= HIS ty (vidx e).
+    Proof.
+      reflexivity.
+    Qed.
+
+    (* Prepend a vtype to the list of variable types of an environment. *)
+    Definition map_prepend_vtype (ty : T) (types : list T)
+               (m : VM.t (entry types)) : VM.t (entry (ty::types)) :=
+      VM.map (prepend_vtype ty (types:=types)) m.
+
+    (* Declare a variable in an environment. *)
+    Program Definition add (v : var) (ty : T) (E : t) : t :=
+      {| vtypes := ty::(vtypes E);
+         vmap := VM.add v {| vty := ty; vidx := HI0 ty (vtypes E) |}
+                        (map_prepend_vtype ty (vmap E)) |}.
+    Next Obligation.
+      case Hxv: (x == v); move/idP: Hxv => Hxv.
+      - (* x == v *)
+        case Hyv: (y == v); move/idP: Hyv => Hyv.
+        + (* y == v *)
+          rewrite (eqP Hxv) (eqP Hyv) in H1.
+          apply: False_ind; apply: (negP H1); reflexivity.
+        + (* y != v *)
+          rewrite (VM.Lemmas.find_add_eq _ _ (Hxv)) in H;
+            rewrite (VM.Lemmas.find_add_neq _ _ Hyv) /prepend_vtype in H0 =>
+          {H1 Hxv Hyv}.
+          case: H => H; rewrite -H /= => {H}.
+          move: (VM.Lemmas.find_map_some H0) => {H0} [ey' [He_ey _]].
+          rewrite He_ey /prepend_vtype /=.
+          move=> Heq; by inversion Heq.
+      - (* x != v *)
+        rewrite (VM.Lemmas.find_add_neq _ _ Hxv) /prepend_vtype in H => {Hxv}.
+        move: (VM.Lemmas.find_map_some H) => {H} [ex' [He_ex He_x]].
+        rewrite He_ex /prepend_vtype /= => {He_ex}.
+        case Hyv: (y == v); move/idP: Hyv => Hyv.
+        + (* y == v *)
+          rewrite (VM.Lemmas.find_add_eq _ _ Hyv) in H0 => {Hyv}.
+          case: H0 => H0; rewrite -H0 /= => {H0}.
+          move=> Heq; by inversion Heq.
+        + (* y != v *)
+          rewrite (VM.Lemmas.find_add_neq _ _ Hyv) /prepend_vtype in H0 => {Hyv}.
+          move: (VM.Lemmas.find_map_some H0) => {H0} [ey' [He_ey He_y]].
+          rewrite He_ey /prepend_vtype /= => {He_ey}.
+          move: (lidx_disjoint He_x He_y H1) => Hne Heq; apply: Hne.
+          exact: (his_eq_lidx_eq Heq).
+    Qed.
+
+    Lemma mem_add_eq :
+      forall (E : t) (x : var) (ty : T), mem x (add x ty E).
+    Proof.
+      move=> E x t. exact: VM.Lemmas.add_eq_b.
+    Qed.
+
+    Lemma mem_prepend_vtype E x t :
+      VM.mem x (map_prepend_vtype t (vmap E)) = VM.mem x (vmap E).
+    Proof.
+      rewrite /map_prepend_vtype. exact: VM.Lemmas.mem_map.
+    Qed.
+
+    Lemma mem_add_neq :
+      forall (E : t) (x y : var) (ty : T), x != y -> mem x (add y ty E) = mem x E.
+    Proof.
+      move=> E x y t Hne. rewrite /mem /add /=. move/negP: Hne => Hne.
+      rewrite (VM.Lemmas.mem_add_neq _ _ Hne).
+      exact: mem_prepend_vtype.
+    Qed.
+
+    Lemma find_add_eq' :
+      forall (E : t) (x : var) (ty : T),
+        find x (add x ty E) = Some {| vty := ty; vidx := HI0 ty (vtypes E) |}.
+    Proof.
+      rewrite /find /add /= => E x ty. rewrite (VM.Lemmas.find_add_eq _ _ (eqxx x)).
+      reflexivity.
+    Qed.
+
+    Lemma find_add_heq :
+      forall (E : t) (x : var) (ty : T),
+        (exists e : entry (ty::(vtypes E)),
+            find x (add x ty E) ~= Some e /\
+            vty e = ty /\
+            lidx_eq (vidx e) (HI0 ty (vtypes E))).
+    Proof.
+      move=> E x ty. exists ({| vty := ty; vidx := HI0 ty (vtypes E) |}) => /=.
+      rewrite find_add_eq'. repeat split; reflexivity.
+    Qed.
+
+    Lemma find_add_eq :
+      forall (E : t) (x : var) (ty : T),
+        (exists e : entry (vtypes (add x ty E)),
+            find x (add x ty E) = Some e /\
+            vty e = ty /\
+            (vidx e) ~= (HI0 ty (vtypes E))).
+    Proof.
+      move=> E x ty. exists ({| vty := ty; vidx := HI0 ty (vtypes E) |}) => /=.
+      rewrite find_add_eq'. repeat split; reflexivity.
+    Qed.
+
+    Lemma find_add_neq' :
+      forall (E : t) (x y : var) (ty : T),
+        x != y ->
+        find x (add y ty E) = match find x E with
+                              | None => None
+                              | Some e => Some (prepend_vtype ty e)
+                              end.
+    Proof.
+      move=> E x y ty Hne. rewrite /find /add /=. move/idP/negP: Hne => Hne.
+      rewrite (VM.Lemmas.find_add_neq _ _ Hne). rewrite /map_prepend_vtype.
+      case H: (VM.find x (vmap E)).
+      - exact: (VM.Lemmas.find_some_map (prepend_vtype ty) H).
+      - exact: (VM.Lemmas.find_none_map (prepend_vtype ty) H).
+    Qed.
+
+    Lemma find_add_neq :
+      forall (E : t) (x y : var) (ty : T),
+        x != y ->
+        find x (add y ty E) ~= match find x E with
+                               | None => None
+                               | Some e => Some (prepend_vtype ty e)
+                               end.
+    Proof.
+      move=> E x y ty Hne. rewrite -(find_add_neq' _ _ Hne). reflexivity.
+    Qed.
+
+    Lemma find_ty_add_eq :
+      forall (E : t) (x : var) (ty : T),
+        find_ty x (add x ty E) = Some ty.
+    Proof.
+      rewrite /find_ty /find /add /= => E x ty.
+      rewrite (VM.Lemmas.find_add_eq _ _ (eqxx x)) /=. reflexivity.
+    Qed.
+
+    Lemma find_ty_add_neq :
+      forall (E : t) (x y : var) (ty : T),
+        x != y -> find_ty x (add y ty E) = find_ty x E.
+    Proof.
+      rewrite /find_ty /find /add /= => E x y ty Hne. move/idP/negP: Hne => Hne.
+      rewrite (VM.Lemmas.find_add_neq _ _ Hne) /=. rewrite /map_prepend_vtype.
+      case H: (VM.M.find x (VM.map (prepend_vtype ty) (vmap E))).
+      - move: (VM.Lemmas.find_map_some H) => [e [He Hfind]].
+        rewrite Hfind. rewrite He prepend_vtype_vty. reflexivity.
+      - rewrite (VM.Lemmas.find_map_none H). reflexivity.
+    Qed.
+
+    Lemma vtypes_add :
+      forall (E : t) (x : V.t) (ty : T),
+        vtypes (add x ty E) = ty::(vtypes E).
+    Proof.
+      reflexivity.
+    Qed.
+
+    (* A pvar is a variable of a specified type defined in an environment. *)
+    (* Note: The equality of vtypes used here is =, not ==. If == is used, then
+     * we will fail to do dependent destruction.
+     *)
+    Inductive pvar_t (E : t) (ty : T) : Type :=
+    | PVar : forall v e, find v E = Some e -> vty e = ty -> pvar_t E ty.
+
+    Definition pvar := pvar_t.
+    Definition make_pvar := PVar.
+
+    (* Return the variable ID of a pvar. *)
+    Definition pvar_var (E : t) (ty : T) (x : pvar E ty) : var :=
+      match x with
+      | PVar v _ _ _ => v
+      end.
+
+    (* Return the lidx of a pvar in an environment. *)
+    Program Definition pvar_lidx (E : t) (ty : T) (x : pvar E ty) : lidx ty (vtypes E) :=
+      match x with
+      | PVar _ e _ _ => vidx e
+      end.
+
+    (* Lemmas about pvar. *)
+
+    Lemma pvar_vtype_eq (E : t) (ty1 ty2 : T) (x : pvar E ty1) (y : pvar E ty2) :
+      pvar_var x == pvar_var y -> ty1 = ty2.
+    Proof.
+      elim: x => x ex Hex Htx /=.
+      elim: y => y ey Hey Hty /=.
+      move/eqP=> Hxy.
+      rewrite -Hxy Hex in Hey.
+      case: Hey => Hexey; rewrite -Hexey Htx in Hty.
+      exact: Hty.
+    Qed.
+
+    Lemma pvar_lidx_heq (E : t) (tyx tyy : T) (x : pvar E tyx) (y : pvar E tyy) :
+      pvar_var x == pvar_var y -> (pvar_lidx x =i pvar_lidx y)%hlist.
+    Proof.
+      elim: x => x ex Hex Htx /=.
+      elim: y => y ey Hey Hty /=.
+      move/eqP=> Hxy.
+      dependent destruction Htx.
+      dependent destruction Hty.
+      rewrite /=.
+      rewrite -Hxy Hex in Hey.
+      case: Hey => Hey; rewrite Hey.
+      reflexivity.
+    Qed.
+
+    Lemma pvar_lidx_eq (E : t) ty (x y : pvar E ty) :
+      pvar_var x == pvar_var y -> pvar_lidx x = pvar_lidx y.
+    Proof.
+      move=> Hxy.
+      apply: lidx_eq_eq.
+      apply: pvar_lidx_heq.
+      assumption.
+    Qed.
+
+    Lemma pvar_lidx_hneq (E : t) (tyx tyy : T) (x : pvar E tyx) (y : pvar E tyy) :
+      pvar_var x != pvar_var y -> pvar_lidx x <>i pvar_lidx y.
+    Proof.
+      elim: x => x ex Hex Htx.
+      elim: y => y ey Hey Hty.
+      move=> /= Hne.
+      dependent destruction Htx.
+      dependent destruction Hty.
+      rewrite /=.
+      apply: (lidx_disjoint Hex Hey).
+      assumption.
+    Qed.
+
+    Lemma pvar_var_mem :
+      forall (E : t) (ty : T) (x : pvar E ty), mem (pvar_var x) E.
+    Proof.
+      move=> E ty [] v e Hfind Hvty /=. exact: (find_some_mem Hfind).
+    Qed.
+
+    (* Create a new variable. *)
+
+    Definition new_var (E : t) : var := VM.new_key (vmap E).
+
+    Lemma new_var_is_new :
+      forall (E : t), ~~ mem (new_var E) E.
+    Proof.
+      move=> E.
+      exact: (VM.new_key_is_new (vmap E)).
+    Qed.
+
+  End Env.
+
+End MakeHEnv.
