src/Var.v
@@ -3,7 +3,7 @@
 
 From Coq Require Import FMaps FSets ZArith.
 From mathcomp Require Import ssreflect ssrbool eqtype.
-From ssrlib Require Import FMaps FSets ZAriths.
+From ssrlib Require Import SsrOrdered FMaps FSets ZAriths.
 
 Set Implicit Arguments.
 Unset Strict Implicit.
@@ -11,125 +11,25 @@ Import Prenex Implicits.
 
 
 
-Open Scope N_scope.
-
 Definition var : Set := N.
 
-Module VarOrder := NOrder.
-
-(* Variable sets. *)
-
-Module VS.
-  Module FS := FSets.MakeTreeSet(NOrder).
-  Include FS.
-
-  (* Generate a new variable. *)
-  Definition new_var (s : t) : var :=
-    match max_elt s with
-    | Some v => v + 1
-    | None => 0
-    end.
-
-  Lemma new_var_is_new :
-    forall (s : t), ~~ mem (new_var s) s.
+Module VarOrder <: SsrOrderedWithDefaultSucc.
+  Include NOrder.
+  Definition succ := N.succ.
+  Lemma ltb_succ : forall (x : t), ltb x (succ x).
   Proof.
-    move=> s.
-    apply/negP => Hmem.
-    move: (mem_2 Hmem) => {Hmem}.
-    rewrite /new_var.
-    case H: (max_elt s).
-    - move=> Hin.
-      move: (max_elt_2 H Hin) => Hfalse.
-      apply: Hfalse.
-      exact: NltnSn.
-    - move: (max_elt_3 H) => {H} H Hin.
-      move: (H 0) => Hnotin; apply: Hnotin; exact: Hin.
+    move=> x. apply/N.ltb_lt. exact: N.lt_succ_diag_r.
   Qed.
+  Definition default := N0.
+End VarOrder.
 
-End VS.
 
 
+(* Variable sets and maps. *)
 
-(* Variable maps. *)
+Module VS := FSets.MakeTreeSetWithNew VarOrder.
 
-Module VM.
-   Module FM := FMaps.MakeTreeMap(NOrder).
-   Include FM.
-
-   Section Aux.
-
-     Variable elt : Type.
-
-     (* Convert a variable map to a variable set. *)
-     Definition vset (m : M.t elt) : VS.t :=
-       fold (fun x _ s => VS.add x s) m VS.empty.
-
-     Lemma mem_vset E :
-       forall x, mem x E -> VS.mem x (vset E).
-     Proof.
-       rewrite /vset.
-       eapply Lemmas.P.fold_rec.
-       - move=> m Hempty x Hmem.
-         apply: False_ind.
-         exact: (Lemmas.empty_mem Hempty Hmem).
-       - move=> x e m E1 E2 _ _ Hadd Hind y Hmem.
-         case Hyx: (y == x).
-         + exact: (VS.Lemmas.mem_add_eq _ Hyx).
-         + move/negP: Hyx => Hyx.
-           rewrite (VS.Lemmas.mem_add_neq _ Hyx).
-           apply: Hind.
-           move: (Hadd y) => {Hadd}.
-           rewrite (VM.Lemmas.find_add_neq _ _ Hyx) => {Hyx} Hfind.
-           rewrite -(VM.Lemmas.find_eq_mem_eq Hfind).
-           exact: Hmem.
-     Qed.
-
-     (* Generate a new variable. *)
-     Definition new_var (m : t elt) : var :=
-       match FM.Lemmas.max_elt m with
-       | Some (v, _) => v + 1
-       | None => 0
-       end.
-
-     Lemma new_var_is_new :
-       forall (m : t elt), ~~ mem (new_var m) m.
-     Proof.
-       move=> m.
-       apply/negP => Hmem.
-       move: (mem_2 Hmem) => {Hmem}.
-       rewrite /new_var.
-       move: (refl_equal (FM.Lemmas.max_elt m)).
-       move: {2}(FM.Lemmas.max_elt m) => x.
-       destruct x.
-       - destruct p as [x ty].
-         move=> Hmax; rewrite Hmax => Hin.
-         move: (FM.Lemmas.max_elt_Above Hmax) => Habove.
-         have: In (x + 1) (remove x m).
-         + case: Hin => ty1 Hmapsto.
-           exists ty1.
-           apply: (remove_2 _ Hmapsto).
-           move=> {Hmax Habove Hmapsto ty ty1 m} Heq.
-           move: (NltnSn x).
-           rewrite {1}(eqP Heq).
-           rewrite Nltnn.
-           discriminate.
-         + move=> Hin1.
-           move: (Habove _ Hin1) => Hlt.
-           move: (Nltn_trans Hlt (NltnSn x)).
-           rewrite Nltnn.
-           discriminate.
-       - move=> Hmax; rewrite Hmax => Hin.
-         move: (FM.Lemmas.max_elt_Empty Hmax) => Hempty.
-         case: Hin => ty Hmapsto.
-         move: (Hempty 0 ty).
-         apply; assumption.
-     Qed.
-
-   End Aux.
-
-End VM.
-
-Close Scope N_scope.
+Module VM := FMaps.MakeTreeMapWithNew VarOrder.
 
 
 
@@ -137,9 +37,9 @@ Close Scope N_scope.
 
 From ssrlib Require Import SsrOrdered.
 
-Module SSAVarOrder := (MakeProdOrdered VarOrder NOrder).
+Module SSAVarOrder := MakeProdOrdered VarOrder NOrder.
 
-Module SSAVS := FSets.Make SSAVarOrder.
+Module SSAVS := FSets.MakeTreeSet SSAVarOrder.
 
 Module SSAVSLemmas := FSetLemmas SSAVS.
 
